refactored reference operations

src/HOL/Imperative_HOL/Ref.thy
@@ -16,185 +16,175 @@ text {*
 
 subsection {* Primitive layer *}
 
-definition
-  ref_present :: "'a\<Colon>heap ref \<Rightarrow> heap \<Rightarrow> bool" where
-  "ref_present r h \<longleftrightarrow> addr_of_ref r < lim h"
+definition present :: "heap \<Rightarrow> 'a\<Colon>heap ref \<Rightarrow> bool" where
+  "present h r \<longleftrightarrow> addr_of_ref r < lim h"
 
-definition
-  get_ref :: "'a\<Colon>heap ref \<Rightarrow> heap \<Rightarrow> 'a" where
-  "get_ref r h = from_nat (refs h (TYPEREP('a)) (addr_of_ref r))"
+definition get :: "heap \<Rightarrow> 'a\<Colon>heap ref \<Rightarrow> 'a" where
+  "get h = from_nat \<circ> refs h TYPEREP('a) \<circ> addr_of_ref"
 
-definition
-  set_ref :: "'a\<Colon>heap ref \<Rightarrow> 'a \<Rightarrow> heap \<Rightarrow> heap" where
-  "set_ref r x = 
-  refs_update (\<lambda>h. h(TYPEREP('a) := ((h (TYPEREP('a))) (addr_of_ref r:=to_nat x))))"
+definition set :: "'a\<Colon>heap ref \<Rightarrow> 'a \<Rightarrow> heap \<Rightarrow> heap" where
+  "set r x = refs_update
+    (\<lambda>h. h(TYPEREP('a) := ((h (TYPEREP('a))) (addr_of_ref r := to_nat x))))"
 
-definition ref :: "'a \<Rightarrow> heap \<Rightarrow> 'a\<Colon>heap ref \<times> heap" where
-  "ref x h = (let
+definition alloc :: "'a \<Rightarrow> heap \<Rightarrow> 'a\<Colon>heap ref \<times> heap" where
+  "alloc x h = (let
      l = lim h;
-     r = Ref l;
-     h'' = set_ref r x (h\<lparr>lim := l + 1\<rparr>)
-   in (r, h''))"
+     r = Ref l
+   in (r, set r x (h\<lparr>lim := l + 1\<rparr>)))"
 
-definition noteq_refs :: "('a\<Colon>heap) ref \<Rightarrow> ('b\<Colon>heap) ref \<Rightarrow> bool" (infix "=!=" 70) where
+definition noteq :: "'a\<Colon>heap ref \<Rightarrow> 'b\<Colon>heap ref \<Rightarrow> bool" (infix "=!=" 70) where
   "r =!= s \<longleftrightarrow> TYPEREP('a) \<noteq> TYPEREP('b) \<or> addr_of_ref r \<noteq> addr_of_ref s"
 
-lemma noteq_refs_sym: "r =!= s \<Longrightarrow> s =!= r"
-  and unequal_refs [simp]: "r \<noteq> r' \<longleftrightarrow> r =!= r'" -- "same types!"
-  unfolding noteq_refs_def by auto
+lemma noteq_sym: "r =!= s \<Longrightarrow> s =!= r"
+  and unequal [simp]: "r \<noteq> r' \<longleftrightarrow> r =!= r'" -- "same types!"
+  by (auto simp add: noteq_def)
 
-lemma noteq_refs_irrefl: "r =!= r \<Longrightarrow> False"
-  unfolding noteq_refs_def by auto
+lemma noteq_irrefl: "r =!= r \<Longrightarrow> False"
+  by (auto simp add: noteq_def)
 
-lemma present_new_ref: "ref_present r h \<Longrightarrow> r =!= fst (ref v h)"
-  by (simp add: ref_present_def ref_def Let_def noteq_refs_def)
+lemma present_alloc_neq: "present h r \<Longrightarrow> r =!= fst (alloc v h)"
+  by (simp add: present_def alloc_def noteq_def Let_def)
 
-lemma next_ref_fresh [simp]:
-  assumes "(r, h') = ref x h"
-  shows "\<not> ref_present r h"
-  using assms by (cases h) (auto simp add: ref_def ref_present_def Let_def)
+lemma next_fresh [simp]:
+  assumes "(r, h') = alloc x h"
+  shows "\<not> present h r"
+  using assms by (cases h) (auto simp add: alloc_def present_def Let_def)
 
-lemma next_ref_present [simp]:
-  assumes "(r, h') = ref x h"
-  shows "ref_present r h'"
-  using assms by (cases h) (auto simp add: ref_def set_ref_def ref_present_def Let_def)
+lemma next_present [simp]:
+  assumes "(r, h') = alloc x h"
+  shows "present h' r"
+  using assms by (cases h) (auto simp add: alloc_def set_def present_def Let_def)
 
-lemma ref_get_set_eq [simp]: "get_ref r (set_ref r x h) = x"
-  by (simp add: get_ref_def set_ref_def)
+lemma get_set_eq [simp]:
+  "get (set r x h) r = x"
+  by (simp add: get_def set_def)
 
-lemma ref_get_set_neq [simp]: "r =!= s \<Longrightarrow> get_ref r (set_ref s x h) = get_ref r h"
-  by (simp add: noteq_refs_def get_ref_def set_ref_def)
+lemma get_set_neq [simp]:
+  "r =!= s \<Longrightarrow> get (set s x h) r = get h r"
+  by (simp add: noteq_def get_def set_def)
 
-(* FIXME: We need some infrastructure to infer that locally generated
-  new refs (by new_ref(_no_init), new_array(')) are distinct
-  from all existing refs.
-*)
+lemma set_same [simp]:
+  "set r x (set r y h) = set r x h"
+  by (simp add: set_def)
 
-lemma ref_set_get: "set_ref r (get_ref r h) h = h"
-apply (simp add: set_ref_def get_ref_def)
-oops
+lemma set_set_swap:
+  "r =!= r' \<Longrightarrow> set r x (set r' x' h) = set r' x' (set r x h)"
+  by (simp add: noteq_def set_def expand_fun_eq)
 
-lemma set_ref_same[simp]:
-  "set_ref r x (set_ref r y h) = set_ref r x h"
-  by (simp add: set_ref_def)
+lemma alloc_set:
+  "fst (alloc x (set r x' h)) = fst (alloc x h)"
+  by (simp add: alloc_def set_def Let_def)
 
-lemma ref_set_set_swap:
-  "r =!= r' \<Longrightarrow> set_ref r x (set_ref r' x' h) = set_ref r' x' (set_ref r x h)"
-  by (simp add: Let_def expand_fun_eq noteq_refs_def set_ref_def)
+lemma get_alloc [simp]:
+  "get (snd (alloc x h)) (fst (alloc x' h)) = x"
+  by (simp add: alloc_def Let_def)
 
-lemma ref_new_set: "fst (ref v (set_ref r v' h)) = fst (ref v h)"
-  by (simp add: ref_def set_ref_def Let_def)
+lemma set_alloc [simp]:
+  "set (fst (alloc v h)) v' (snd (alloc v h)) = snd (alloc v' h)"
+  by (simp add: alloc_def Let_def)
 
-lemma ref_get_new [simp]:
-  "get_ref (fst (ref v h)) (snd (ref v' h)) = v'"
-  by (simp add: ref_def Let_def split_def)
+lemma get_alloc_neq: "r =!= fst (alloc v h) \<Longrightarrow> 
+  get (snd (alloc v h)) r  = get h r"
+  by (simp add: get_def set_def alloc_def Let_def noteq_def)
 
-lemma ref_set_new [simp]:
-  "set_ref (fst (ref v h)) new_v (snd (ref v h)) = snd (ref new_v h)"
-  by (simp add: ref_def Let_def split_def)
+lemma lim_set [simp]:
+  "lim (set r v h) = lim h"
+  by (simp add: set_def)
 
-lemma ref_get_new_neq: "r =!= (fst (ref v h)) \<Longrightarrow> 
-  get_ref r (snd (ref v h)) = get_ref r h"
-  by (simp add: get_ref_def set_ref_def ref_def Let_def noteq_refs_def)
+lemma present_alloc [simp]: 
+  "present h r \<Longrightarrow> present (snd (alloc v h)) r"
+  by (simp add: present_def alloc_def Let_def)
 
-lemma lim_set_ref [simp]:
-  "lim (set_ref r v h) = lim h"
-  by (simp add: set_ref_def)
+lemma present_set [simp]:
+  "present (set r v h) = present h"
+  by (simp add: present_def expand_fun_eq)
 
-lemma ref_present_new_ref [simp]: 
-  "ref_present r h \<Longrightarrow> ref_present r (snd (ref v h))"
-  by (simp add: ref_present_def ref_def Let_def)
-
-lemma ref_present_set_ref [simp]:
-  "ref_present r (set_ref r' v h) = ref_present r h"
-  by (simp add: set_ref_def ref_present_def)
-
-lemma noteq_refsI: "\<lbrakk> ref_present r h; \<not>ref_present r' h \<rbrakk>  \<Longrightarrow> r =!= r'"
-  unfolding noteq_refs_def ref_present_def
-  by auto
+lemma noteq_I:
+  "present h r \<Longrightarrow> \<not> present h r' \<Longrightarrow> r =!= r'"
+  by (auto simp add: noteq_def present_def)
 
 
 subsection {* Primitives *}
 
-definition
-  new :: "'a\<Colon>heap \<Rightarrow> 'a ref Heap" where
-  [code del]: "new v = Heap_Monad.heap (Ref.ref v)"
+definition ref :: "'a\<Colon>heap \<Rightarrow> 'a ref Heap" where
+  [code del]: "ref v = Heap_Monad.heap (alloc v)"
 
-definition
-  lookup :: "'a\<Colon>heap ref \<Rightarrow> 'a Heap" ("!_" 61) where
-  [code del]: "lookup r = Heap_Monad.heap (\<lambda>h. (get_ref r h, h))"
+definition lookup :: "'a\<Colon>heap ref \<Rightarrow> 'a Heap" ("!_" 61) where
+  [code del]: "lookup r = Heap_Monad.heap (\<lambda>h. (get h r, h))"
 
-definition
-  update :: "'a ref \<Rightarrow> ('a\<Colon>heap) \<Rightarrow> unit Heap" ("_ := _" 62) where
-  [code del]: "update r e = Heap_Monad.heap (\<lambda>h. ((), set_ref r e h))"
+definition update :: "'a ref \<Rightarrow> 'a\<Colon>heap \<Rightarrow> unit Heap" ("_ := _" 62) where
+  [code del]: "update r v = Heap_Monad.heap (\<lambda>h. ((), set r v h))"
 
 
 subsection {* Derivates *}
 
-definition
-  change :: "('a\<Colon>heap \<Rightarrow> 'a) \<Rightarrow> 'a ref \<Rightarrow> 'a Heap"
-where
-  "change f r = (do x \<leftarrow> ! r;
-                    let y = f x;
-                    r := y;
-                    return y
-                 done)"
-
-hide_const (open) new lookup update change
+definition change :: "('a\<Colon>heap \<Rightarrow> 'a) \<Rightarrow> 'a ref \<Rightarrow> 'a Heap" where
+  "change f r = (do
+     x \<leftarrow> ! r;
+     let y = f x;
+     r := y;
+     return y
+   done)"
 
 
 subsection {* Properties *}
 
 lemma lookup_chain:
   "(!r \<guillemotright> f) = f"
-  by (cases f)
-    (auto simp add: Let_def bindM_def lookup_def expand_fun_eq)
+  by (rule Heap_eqI) (simp add: lookup_def)
 
 lemma update_change [code]:
-  "r := e = Ref.change (\<lambda>_. e) r \<guillemotright> return ()"
-  by (auto simp add: change_def lookup_chain)
+  "r := e = change (\<lambda>_. e) r \<guillemotright> return ()"
+  by (rule Heap_eqI) (simp add: change_def lookup_chain)
 
 
 text {* Non-interaction between imperative array and imperative references *}
 
-lemma get_array_set_ref [simp]: "get_array a (set_ref r v h) = get_array a h"
-  by (simp add: get_array_def set_ref_def)
+lemma get_array_set [simp]:
+  "get_array a (set r v h) = get_array a h"
+  by (simp add: get_array_def set_def)
 
-lemma nth_set_ref [simp]: "get_array a (set_ref r v h) ! i = get_array a h ! i"
+lemma nth_set [simp]:
+  "get_array a (set r v h) ! i = get_array a h ! i"
   by simp
 
-lemma get_ref_upd [simp]: "get_ref r (Array.change a i v h) = get_ref r h"
-  by (simp add: get_ref_def set_array_def Array.change_def)
+lemma get_change [simp]:
+  "get (Array.change a i v h) r  = get h r"
+  by (simp add: get_def Array.change_def set_array_def)
 
-lemma new_ref_upd: "fst (ref v (Array.change a i v' h)) = fst (ref v h)"
-  by (simp add: set_array_def get_array_def Let_def ref_new_set Array.change_def ref_def)
+lemma alloc_change:
+  "fst (alloc v (Array.change a i v' h)) = fst (alloc v h)"
+  by (simp add: Array.change_def get_array_def set_array_def alloc_def Let_def)
 
-lemma upd_set_ref_swap: "Array.change a i v (set_ref r v' h) = set_ref r v' (Array.change a i v h)"
-  by (simp add: set_ref_def Array.change_def get_array_def set_array_def)
+lemma change_set_swap:
+  "Array.change a i v (set r v' h) = set r v' (Array.change a i v h)"
+  by (simp add: Array.change_def get_array_def set_array_def set_def)
 
-lemma length_new_ref[simp]: 
-  "length a (snd (ref v h)) = length a h"
-  by (simp add: get_array_def set_ref_def length_def  ref_def Let_def)
+lemma length_alloc [simp]: 
+  "Array.length a (snd (alloc v h)) = Array.length a h"
+  by (simp add: Array.length_def get_array_def alloc_def set_def Let_def)
 
-lemma get_array_new_ref [simp]: 
-  "get_array a (snd (ref v h)) = get_array a h"
-  by (simp add: ref_def set_ref_def get_array_def Let_def)
+lemma get_array_alloc [simp]: 
+  "get_array a (snd (alloc v h)) = get_array a h"
+  by (simp add: get_array_def alloc_def set_def Let_def)
 
-lemma ref_present_upd [simp]: 
-  "ref_present r (Array.change a i v h) = ref_present r h"
-  by (simp add: Array.change_def ref_present_def set_array_def get_array_def)
+lemma present_change [simp]: 
+  "present (Array.change a i v h) = present h"
+  by (simp add: Array.change_def set_array_def expand_fun_eq present_def)
 
-lemma array_present_set_ref [simp]:
-  "array_present a (set_ref r v h) = array_present a h"
-  by (simp add: array_present_def set_ref_def)
+lemma array_present_set [simp]:
+  "array_present a (set r v h) = array_present a h"
+  by (simp add: array_present_def set_def)
 
-lemma array_present_new_ref [simp]:
-  "array_present a h \<Longrightarrow> array_present a (snd (ref v h))"
-  by (simp add: array_present_def ref_def Let_def)
+lemma array_present_alloc [simp]:
+  "array_present a h \<Longrightarrow> array_present a (snd (alloc v h))"
+  by (simp add: array_present_def alloc_def Let_def)
 
-lemma array_ref_set_set_swap:
-  "set_array r x (set_ref r' x' h) = set_ref r' x' (set_array r x h)"
-  by (simp add: Let_def expand_fun_eq set_array_def set_ref_def)
+lemma set_array_set_swap:
+  "set_array a xs (set r x' h) = set r x' (set_array a xs h)"
+  by (simp add: set_array_def set_def)
+
+hide_const (open) present get set alloc lookup update change
 
 
 subsection {* Code generator setup *}
@@ -203,7 +193,7 @@ subsubsection {* SML *}
 
 code_type ref (SML "_/ Unsynchronized.ref")
 code_const Ref (SML "raise/ (Fail/ \"bare Ref\")")
-code_const Ref.new (SML "(fn/ ()/ =>/ Unsynchronized.ref/ _)")
+code_const ref (SML "(fn/ ()/ =>/ Unsynchronized.ref/ _)")
 code_const Ref.lookup (SML "(fn/ ()/ =>/ !/ _)")
 code_const Ref.update (SML "(fn/ ()/ =>/ _/ :=/ _)")
 
@@ -214,7 +204,7 @@ subsubsection {* OCaml *}
 
 code_type ref (OCaml "_/ ref")
 code_const Ref (OCaml "failwith/ \"bare Ref\")")
-code_const Ref.new (OCaml "(fn/ ()/ =>/ ref/ _)")
+code_const ref (OCaml "(fn/ ()/ =>/ ref/ _)")
 code_const Ref.lookup (OCaml "(fn/ ()/ =>/ !/ _)")
 code_const Ref.update (OCaml "(fn/ ()/ =>/ _/ :=/ _)")
 
@@ -225,7 +215,7 @@ subsubsection {* Haskell *}
 
 code_type ref (Haskell "Heap.STRef/ Heap.RealWorld/ _")
 code_const Ref (Haskell "error/ \"bare Ref\"")
-code_const Ref.new (Haskell "Heap.newSTRef")
+code_const ref (Haskell "Heap.newSTRef")
 code_const Ref.lookup (Haskell "Heap.readSTRef")
 code_const Ref.update (Haskell "Heap.writeSTRef")
 
