src/HOL/Imperative_HOL/ex/Linked_Lists.thy
@@ -13,7 +13,7 @@ section {* Definition of Linked Lists *}
 setup {* Sign.add_const_constraint (@{const_name Ref}, SOME @{typ "nat \<Rightarrow> 'a\<Colon>type ref"}) *}
 datatype 'a node = Empty | Node 'a "('a node) ref"
 
-fun
+primrec
   node_encode :: "'a\<Colon>countable node \<Rightarrow> nat"
 where
   "node_encode Empty = 0"
@@ -28,11 +28,11 @@ qed
 
 instance node :: (heap) heap ..
 
-fun make_llist :: "'a\<Colon>heap list \<Rightarrow> 'a node Heap"
+primrec make_llist :: "'a\<Colon>heap list \<Rightarrow> 'a node Heap"
 where 
   [simp del]: "make_llist []     = return Empty"
             | "make_llist (x#xs) = do tl   \<leftarrow> make_llist xs;
-                                      next \<leftarrow> Ref.new tl;
+                                      next \<leftarrow> ref tl;
                                       return (Node x next)
                                    done"
 
@@ -63,24 +63,24 @@ section {* Proving correctness with relational abstraction *}
 
 subsection {* Definition of list_of, list_of', refs_of and refs_of' *}
 
-fun list_of :: "heap \<Rightarrow> ('a::heap) node \<Rightarrow> 'a list \<Rightarrow> bool"
+primrec list_of :: "heap \<Rightarrow> ('a::heap) node \<Rightarrow> 'a list \<Rightarrow> bool"
 where
   "list_of h r [] = (r = Empty)"
-| "list_of h r (a#as) = (case r of Empty \<Rightarrow> False | Node b bs \<Rightarrow> (a = b \<and> list_of h (get_ref bs h) as))"
+| "list_of h r (a#as) = (case r of Empty \<Rightarrow> False | Node b bs \<Rightarrow> (a = b \<and> list_of h (Ref.get h bs) as))"
  
 definition list_of' :: "heap \<Rightarrow> ('a::heap) node ref \<Rightarrow> 'a list \<Rightarrow> bool"
 where
-  "list_of' h r xs = list_of h (get_ref r h) xs"
+  "list_of' h r xs = list_of h (Ref.get h r) xs"
 
-fun refs_of :: "heap \<Rightarrow> ('a::heap) node \<Rightarrow> 'a node ref list \<Rightarrow> bool"
+primrec refs_of :: "heap \<Rightarrow> ('a::heap) node \<Rightarrow> 'a node ref list \<Rightarrow> bool"
 where
   "refs_of h r [] = (r = Empty)"
-| "refs_of h r (x#xs) = (case r of Empty \<Rightarrow> False | Node b bs \<Rightarrow> (x = bs) \<and> refs_of h (get_ref bs h) xs)"
+| "refs_of h r (x#xs) = (case r of Empty \<Rightarrow> False | Node b bs \<Rightarrow> (x = bs) \<and> refs_of h (Ref.get h bs) xs)"
 
-fun refs_of' :: "heap \<Rightarrow> ('a::heap) node ref \<Rightarrow> 'a node ref list \<Rightarrow> bool"
+primrec refs_of' :: "heap \<Rightarrow> ('a::heap) node ref \<Rightarrow> 'a node ref list \<Rightarrow> bool"
 where
   "refs_of' h r [] = False"
-| "refs_of' h r (x#xs) = ((x = r) \<and> refs_of h (get_ref x h) xs)"
+| "refs_of' h r (x#xs) = ((x = r) \<and> refs_of h (Ref.get h x) xs)"
 
 
 subsection {* Properties of these definitions *}
@@ -88,35 +88,35 @@ subsection {* Properties of these definitions *}
 lemma list_of_Empty[simp]: "list_of h Empty xs = (xs = [])"
 by (cases xs, auto)
 
-lemma list_of_Node[simp]: "list_of h (Node x ps) xs = (\<exists>xs'. (xs = x # xs') \<and> list_of h (get_ref ps h) xs')"
+lemma list_of_Node[simp]: "list_of h (Node x ps) xs = (\<exists>xs'. (xs = x # xs') \<and> list_of h (Ref.get h ps) xs')"
 by (cases xs, auto)
 
-lemma list_of'_Empty[simp]: "get_ref q h = Empty \<Longrightarrow> list_of' h q xs = (xs = [])"
+lemma list_of'_Empty[simp]: "Ref.get h q = Empty \<Longrightarrow> list_of' h q xs = (xs = [])"
 unfolding list_of'_def by simp
 
-lemma list_of'_Node[simp]: "get_ref q h = Node x ps \<Longrightarrow> list_of' h q xs = (\<exists>xs'. (xs = x # xs') \<and> list_of' h ps xs')"
+lemma list_of'_Node[simp]: "Ref.get h q = Node x ps \<Longrightarrow> list_of' h q xs = (\<exists>xs'. (xs = x # xs') \<and> list_of' h ps xs')"
 unfolding list_of'_def by simp
 
-lemma list_of'_Nil: "list_of' h q [] \<Longrightarrow> get_ref q h = Empty"
+lemma list_of'_Nil: "list_of' h q [] \<Longrightarrow> Ref.get h q = Empty"
 unfolding list_of'_def by simp
 
 lemma list_of'_Cons: 
 assumes "list_of' h q (x#xs)"
-obtains n where "get_ref q h = Node x n" and "list_of' h n xs"
+obtains n where "Ref.get h q = Node x n" and "list_of' h n xs"
 using assms unfolding list_of'_def by (auto split: node.split_asm)
 
 lemma refs_of_Empty[simp] : "refs_of h Empty xs = (xs = [])"
   by (cases xs, auto)
 
-lemma refs_of_Node[simp]: "refs_of h (Node x ps) xs = (\<exists>prs. xs = ps # prs \<and> refs_of h (get_ref ps h) prs)"
+lemma refs_of_Node[simp]: "refs_of h (Node x ps) xs = (\<exists>prs. xs = ps # prs \<and> refs_of h (Ref.get h ps) prs)"
   by (cases xs, auto)
 
-lemma refs_of'_def': "refs_of' h p ps = (\<exists>prs. (ps = (p # prs)) \<and> refs_of h (get_ref p h) prs)"
+lemma refs_of'_def': "refs_of' h p ps = (\<exists>prs. (ps = (p # prs)) \<and> refs_of h (Ref.get h p) prs)"
 by (cases ps, auto)
 
 lemma refs_of'_Node:
   assumes "refs_of' h p xs"
-  assumes "get_ref p h = Node x pn"
+  assumes "Ref.get h p = Node x pn"
   obtains pnrs
   where "xs = p # pnrs" and "refs_of' h pn pnrs"
 using assms
@@ -166,7 +166,7 @@ lemma list_of'_refs_of'_HOL:
   assumes "list_of' h r xs"
   shows "\<exists>rs. refs_of' h r rs"
 proof -
-  from assms obtain rs' where "refs_of h (get_ref r h) rs'"
+  from assms obtain rs' where "refs_of h (Ref.get h r) rs'"
     unfolding list_of'_def by (rule list_of_refs_of)
   thus ?thesis unfolding refs_of'_def' by auto
 qed
@@ -238,7 +238,7 @@ apply auto
 done
 
 lemma refs_of_next:
-assumes "refs_of h (get_ref p h) rs"
+assumes "refs_of h (Ref.get h p) rs"
   shows "p \<notin> set rs"
 proof (rule ccontr)
   assume a: "\<not> (p \<notin> set rs)"
@@ -264,7 +264,7 @@ lemma refs_of'_distinct: "refs_of' h p rs \<Longrightarrow> distinct rs"
 
 subsection {* Interaction of these predicates with our heap transitions *}
 
-lemma list_of_set_ref: "refs_of h q rs \<Longrightarrow> p \<notin> set rs \<Longrightarrow> list_of (set_ref p v h) q as = list_of h q as"
+lemma list_of_set_ref: "refs_of h q rs \<Longrightarrow> p \<notin> set rs \<Longrightarrow> list_of (Ref.set p v h) q as = list_of h q as"
 using assms
 proof (induct as arbitrary: q rs)
   case Nil thus ?case by simp
@@ -275,15 +275,15 @@ next
     case Empty thus ?thesis by auto
   next
     case (Node a ref)
-    from Cons(2) Node obtain rs' where 1: "refs_of h (get_ref ref h) rs'" and rs_rs': "rs = ref # rs'" by auto
+    from Cons(2) Node obtain rs' where 1: "refs_of h (Ref.get h ref) rs'" and rs_rs': "rs = ref # rs'" by auto
     from Cons(3) rs_rs' have "ref \<noteq> p" by fastsimp
-    hence ref_eq: "get_ref ref (set_ref p v h) = (get_ref ref h)" by (auto simp add: ref_get_set_neq)
+    hence ref_eq: "Ref.get (Ref.set p v h) ref = (Ref.get h ref)" by (auto simp add: Ref.get_set_neq)
     from rs_rs' Cons(3) have 2: "p \<notin> set rs'" by simp
     from Cons.hyps[OF 1 2] Node ref_eq show ?thesis by simp
   qed
 qed
 
-lemma refs_of_set_ref: "refs_of h q rs \<Longrightarrow> p \<notin> set rs \<Longrightarrow> refs_of (set_ref p v h) q as = refs_of h q as"
+lemma refs_of_set_ref: "refs_of h q rs \<Longrightarrow> p \<notin> set rs \<Longrightarrow> refs_of (Ref.set p v h) q as = refs_of h q as"
 proof (induct as arbitrary: q rs)
   case Nil thus ?case by simp
 next
@@ -293,15 +293,15 @@ next
     case Empty thus ?thesis by auto
   next
     case (Node a ref)
-    from Cons(2) Node obtain rs' where 1: "refs_of h (get_ref ref h) rs'" and rs_rs': "rs = ref # rs'" by auto
+    from Cons(2) Node obtain rs' where 1: "refs_of h (Ref.get h ref) rs'" and rs_rs': "rs = ref # rs'" by auto
     from Cons(3) rs_rs' have "ref \<noteq> p" by fastsimp
-    hence ref_eq: "get_ref ref (set_ref p v h) = (get_ref ref h)" by (auto simp add: ref_get_set_neq)
+    hence ref_eq: "Ref.get (Ref.set p v h) ref = (Ref.get h ref)" by (auto simp add: Ref.get_set_neq)
     from rs_rs' Cons(3) have 2: "p \<notin> set rs'" by simp
     from Cons.hyps[OF 1 2] Node ref_eq show ?thesis by auto
   qed
 qed
 
-lemma refs_of_set_ref2: "refs_of (set_ref p v h) q rs \<Longrightarrow> p \<notin> set rs \<Longrightarrow> refs_of (set_ref p v h) q rs = refs_of h q rs"
+lemma refs_of_set_ref2: "refs_of (Ref.set p v h) q rs \<Longrightarrow> p \<notin> set rs \<Longrightarrow> refs_of (Ref.set p v h) q rs = refs_of h q rs"
 proof (induct rs arbitrary: q)
   case Nil thus ?case by simp
 next
@@ -311,9 +311,9 @@ next
     case Empty thus ?thesis by auto
   next
     case (Node a ref)
-    from Cons(2) Node have 1:"refs_of (set_ref p v h) (get_ref ref (set_ref p v h)) xs" and x_ref: "x = ref" by auto
+    from Cons(2) Node have 1:"refs_of (Ref.set p v h) (Ref.get (Ref.set p v h) ref) xs" and x_ref: "x = ref" by auto
     from Cons(3) this have "ref \<noteq> p" by fastsimp
-    hence ref_eq: "get_ref ref (set_ref p v h) = (get_ref ref h)" by (auto simp add: ref_get_set_neq)
+    hence ref_eq: "Ref.get (Ref.set p v h) ref = (Ref.get h ref)" by (auto simp add: Ref.get_set_neq)
     from Cons(3) have 2: "p \<notin> set xs" by simp
     with Cons.hyps 1 2 Node ref_eq show ?thesis
       by simp
@@ -323,7 +323,7 @@ qed
 lemma list_of'_set_ref:
   assumes "refs_of' h q rs"
   assumes "p \<notin> set rs"
-  shows "list_of' (set_ref p v h) q as = list_of' h q as"
+  shows "list_of' (Ref.set p v h) q as = list_of' h q as"
 proof -
   from assms have "q \<noteq> p" by (auto simp only: dest!: refs_of'E)
   with assms show ?thesis
@@ -333,18 +333,18 @@ qed
 
 lemma list_of'_set_next_ref_Node[simp]:
   assumes "list_of' h r xs"
-  assumes "get_ref p h = Node x r'"
+  assumes "Ref.get h p = Node x r'"
   assumes "refs_of' h r rs"
   assumes "p \<notin> set rs"
-  shows "list_of' (set_ref p (Node x r) h) p (x#xs) = list_of' h r xs"
+  shows "list_of' (Ref.set p (Node x r) h) p (x#xs) = list_of' h r xs"
 using assms
 unfolding list_of'_def refs_of'_def'
-by (auto simp add: list_of_set_ref noteq_refs_sym)
+by (auto simp add: list_of_set_ref Ref.noteq_sym)
 
 lemma refs_of'_set_ref:
   assumes "refs_of' h q rs"
   assumes "p \<notin> set rs"
-  shows "refs_of' (set_ref p v h) q as = refs_of' h q as"
+  shows "refs_of' (Ref.set p v h) q as = refs_of' h q as"
 using assms
 proof -
   from assms have "q \<noteq> p" by (auto simp only: dest!: refs_of'E)
@@ -354,9 +354,9 @@ proof -
 qed
 
 lemma refs_of'_set_ref2:
-  assumes "refs_of' (set_ref p v h) q rs"
+  assumes "refs_of' (Ref.set p v h) q rs"
   assumes "p \<notin> set rs"
-  shows "refs_of' (set_ref p v h) q as = refs_of' h q as"
+  shows "refs_of' (Ref.set p v h) q as = refs_of' h q as"
 using assms
 proof -
   from assms have "q \<noteq> p" by (auto simp only: dest!: refs_of'E)
@@ -364,7 +364,7 @@ proof -
     unfolding refs_of'_def'
     apply auto
     apply (subgoal_tac "prs = prsa")
-    apply (insert refs_of_set_ref2[of p v h "get_ref q h"])
+    apply (insert refs_of_set_ref2[of p v h "Ref.get h q"])
     apply (erule_tac x="prs" in meta_allE)
     apply auto
     apply (auto dest: refs_of_is_fun)
@@ -372,15 +372,15 @@ proof -
 qed
 
 lemma refs_of'_set_next_ref:
-assumes "get_ref p h1 = Node x pn"
-assumes "refs_of' (set_ref p (Node x r1) h1) p rs"
+assumes "Ref.get h1 p = Node x pn"
+assumes "refs_of' (Ref.set p (Node x r1) h1) p rs"
 obtains r1s where "rs = (p#r1s)" and "refs_of' h1 r1 r1s"
 using assms
 proof -
   from assms refs_of'_distinct[OF assms(2)] have "\<exists> r1s. rs = (p # r1s) \<and> refs_of' h1 r1 r1s"
     apply -
     unfolding refs_of'_def'[of _ p]
-    apply (auto, frule refs_of_set_ref2) by (auto dest: noteq_refs_sym)
+    apply (auto, frule refs_of_set_ref2) by (auto dest: Ref.noteq_sym)
   with prems show thesis by auto
 qed
 
@@ -388,7 +388,7 @@ section {* Proving make_llist and traverse correct *}
 
 lemma refs_of_invariant:
   assumes "refs_of h (r::('a::heap) node) xs"
-  assumes "\<forall>refs. refs_of h r refs \<longrightarrow> (\<forall>ref \<in> set refs. ref_present ref h \<and> ref_present ref h' \<and> get_ref ref h = get_ref ref h')"
+  assumes "\<forall>refs. refs_of h r refs \<longrightarrow> (\<forall>ref \<in> set refs. Ref.present h ref \<and> Ref.present h' ref \<and> Ref.get h ref = Ref.get h' ref)"
   shows "refs_of h' r xs"
 using assms
 proof (induct xs arbitrary: r)
@@ -396,28 +396,28 @@ proof (induct xs arbitrary: r)
 next
   case (Cons x xs')
   from Cons(2) obtain v where Node: "r = Node v x" by (cases r, auto)
-  from Cons(2) Node have refs_of_next: "refs_of h (get_ref x h) xs'" by simp
-  from Cons(2-3) Node have ref_eq: "get_ref x h = get_ref x h'" by auto
-  from ref_eq refs_of_next have 1: "refs_of h (get_ref x h') xs'" by simp
-  from Cons(2) Cons(3) have "\<forall>ref \<in> set xs'. ref_present ref h \<and> ref_present ref h' \<and> get_ref ref h = get_ref ref h'"
+  from Cons(2) Node have refs_of_next: "refs_of h (Ref.get h x) xs'" by simp
+  from Cons(2-3) Node have ref_eq: "Ref.get h x = Ref.get h' x" by auto
+  from ref_eq refs_of_next have 1: "refs_of h (Ref.get h' x) xs'" by simp
+  from Cons(2) Cons(3) have "\<forall>ref \<in> set xs'. Ref.present h ref \<and> Ref.present h' ref \<and> Ref.get h ref = Ref.get h' ref"
     by fastsimp
-  with Cons(3) 1 have 2: "\<forall>refs. refs_of h (get_ref x h') refs \<longrightarrow> (\<forall>ref \<in> set refs. ref_present ref h \<and> ref_present ref h' \<and> get_ref ref h = get_ref ref h')"
+  with Cons(3) 1 have 2: "\<forall>refs. refs_of h (Ref.get h' x) refs \<longrightarrow> (\<forall>ref \<in> set refs. Ref.present h ref \<and> Ref.present h' ref \<and> Ref.get h ref = Ref.get h' ref)"
     by (fastsimp dest: refs_of_is_fun)
-  from Cons.hyps[OF 1 2] have "refs_of h' (get_ref x h') xs'" .
+  from Cons.hyps[OF 1 2] have "refs_of h' (Ref.get h' x) xs'" .
   with Node show ?case by simp
 qed
 
 lemma refs_of'_invariant:
   assumes "refs_of' h r xs"
-  assumes "\<forall>refs. refs_of' h r refs \<longrightarrow> (\<forall>ref \<in> set refs. ref_present ref h \<and> ref_present ref h' \<and> get_ref ref h = get_ref ref h')"
+  assumes "\<forall>refs. refs_of' h r refs \<longrightarrow> (\<forall>ref \<in> set refs. Ref.present h ref \<and> Ref.present h' ref \<and> Ref.get h ref = Ref.get h' ref)"
   shows "refs_of' h' r xs"
 using assms
 proof -
-  from assms obtain prs where refs:"refs_of h (get_ref r h) prs" and xs_def: "xs = r # prs"
+  from assms obtain prs where refs:"refs_of h (Ref.get h r) prs" and xs_def: "xs = r # prs"
     unfolding refs_of'_def' by auto
-  from xs_def assms have x_eq: "get_ref r h = get_ref r h'" by fastsimp
-  from refs assms xs_def have 2: "\<forall>refs. refs_of h (get_ref r h) refs \<longrightarrow>
-     (\<forall>ref\<in>set refs. ref_present ref h \<and> ref_present ref h' \<and> get_ref ref h = get_ref ref h')" 
+  from xs_def assms have x_eq: "Ref.get h r = Ref.get h' r" by fastsimp
+  from refs assms xs_def have 2: "\<forall>refs. refs_of h (Ref.get h r) refs \<longrightarrow>
+     (\<forall>ref\<in>set refs. Ref.present h ref \<and> Ref.present h' ref \<and> Ref.get h ref = Ref.get h' ref)" 
     by (fastsimp dest: refs_of_is_fun)
   from refs_of_invariant [OF refs 2] xs_def x_eq show ?thesis
     unfolding refs_of'_def' by auto
@@ -425,7 +425,7 @@ qed
 
 lemma list_of_invariant:
   assumes "list_of h (r::('a::heap) node) xs"
-  assumes "\<forall>refs. refs_of h r refs \<longrightarrow> (\<forall>ref \<in> set refs. ref_present ref h \<and> ref_present ref h' \<and> get_ref ref h = get_ref ref h')"
+  assumes "\<forall>refs. refs_of h r refs \<longrightarrow> (\<forall>ref \<in> set refs. Ref.present h ref \<and> Ref.present h' ref \<and> Ref.get h ref = Ref.get h' ref)"
   shows "list_of h' r xs"
 using assms
 proof (induct xs arbitrary: r)
@@ -437,16 +437,16 @@ next
     by (cases r, auto)
   from Cons(2) obtain rs where rs_def: "refs_of h r rs" by (rule list_of_refs_of)
   from Node rs_def obtain rss where refs_of: "refs_of h r (ref#rss)" and rss_def: "rs = ref#rss" by auto
-  from Cons(3) Node refs_of have ref_eq: "get_ref ref h = get_ref ref h'"
+  from Cons(3) Node refs_of have ref_eq: "Ref.get h ref = Ref.get h' ref"
     by auto
-  from Cons(2) ref_eq Node have 1: "list_of h (get_ref ref h') xs'" by simp
-  from refs_of Node ref_eq have refs_of_ref: "refs_of h (get_ref ref h') rss" by simp
-  from Cons(3) rs_def have rs_heap_eq: "\<forall>ref\<in>set rs. ref_present ref h \<and> ref_present ref h' \<and> get_ref ref h = get_ref ref h'" by simp
-  from refs_of_ref rs_heap_eq rss_def have 2: "\<forall>refs. refs_of h (get_ref ref h') refs \<longrightarrow>
-          (\<forall>ref\<in>set refs. ref_present ref h \<and> ref_present ref h' \<and> get_ref ref h = get_ref ref h')"
+  from Cons(2) ref_eq Node have 1: "list_of h (Ref.get h' ref) xs'" by simp
+  from refs_of Node ref_eq have refs_of_ref: "refs_of h (Ref.get h' ref) rss" by simp
+  from Cons(3) rs_def have rs_heap_eq: "\<forall>ref\<in>set rs. Ref.present h ref \<and> Ref.present h' ref \<and> Ref.get h ref = Ref.get h' ref" by simp
+  from refs_of_ref rs_heap_eq rss_def have 2: "\<forall>refs. refs_of h (Ref.get h' ref) refs \<longrightarrow>
+          (\<forall>ref\<in>set refs. Ref.present h ref \<and> Ref.present h' ref \<and> Ref.get h ref = Ref.get h' ref)"
     by (auto dest: refs_of_is_fun)
   from Cons(1)[OF 1 2]
-  have "list_of h' (get_ref ref h') xs'" .
+  have "list_of h' (Ref.get h' ref) xs'" .
   with Node show ?case
     unfolding list_of'_def
     by simp
@@ -454,29 +454,29 @@ qed
 
 lemma make_llist:
 assumes "crel (make_llist xs) h h' r"
-shows "list_of h' r xs \<and> (\<forall>rs. refs_of h' r rs \<longrightarrow> (\<forall>ref \<in> (set rs). ref_present ref h'))"
+shows "list_of h' r xs \<and> (\<forall>rs. refs_of h' r rs \<longrightarrow> (\<forall>ref \<in> (set rs). Ref.present h' ref))"
 using assms 
 proof (induct xs arbitrary: h h' r)
   case Nil thus ?case by (auto elim: crel_return simp add: make_llist.simps)
 next
   case (Cons x xs')
   from Cons.prems obtain h1 r1 r' where make_llist: "crel (make_llist xs') h h1 r1"
-    and crel_refnew:"crel (Ref.new r1) h1 h' r'" and Node: "r = Node x r'"
+    and crel_refnew:"crel (ref r1) h1 h' r'" and Node: "r = Node x r'"
     unfolding make_llist.simps
     by (auto elim!: crelE crel_return)
   from Cons.hyps[OF make_llist] have list_of_h1: "list_of h1 r1 xs'" ..
   from Cons.hyps[OF make_llist] obtain rs' where rs'_def: "refs_of h1 r1 rs'" by (auto intro: list_of_refs_of)
-  from Cons.hyps[OF make_llist] rs'_def have refs_present: "\<forall>ref\<in>set rs'. ref_present ref h1" by simp
+  from Cons.hyps[OF make_llist] rs'_def have refs_present: "\<forall>ref\<in>set rs'. Ref.present h1 ref" by simp
   from crel_refnew rs'_def refs_present have refs_unchanged: "\<forall>refs. refs_of h1 r1 refs \<longrightarrow>
-         (\<forall>ref\<in>set refs. ref_present ref h1 \<and> ref_present ref h' \<and> get_ref ref h1 = get_ref ref h')"
-    by (auto elim!: crel_Ref_new dest: refs_of_is_fun)
+         (\<forall>ref\<in>set refs. Ref.present h1 ref \<and> Ref.present h' ref \<and> Ref.get h1 ref = Ref.get h' ref)"
+    by (auto elim!: crel_ref dest: refs_of_is_fun)
   with list_of_invariant[OF list_of_h1 refs_unchanged] Node crel_refnew have fstgoal: "list_of h' r (x # xs')"
     unfolding list_of.simps
-    by (auto elim!: crel_Ref_new)
-  from refs_unchanged rs'_def have refs_still_present: "\<forall>ref\<in>set rs'. ref_present ref h'" by auto
+    by (auto elim!: crel_ref)
+  from refs_unchanged rs'_def have refs_still_present: "\<forall>ref\<in>set rs'. Ref.present h' ref" by auto
   from refs_of_invariant[OF rs'_def refs_unchanged] refs_unchanged Node crel_refnew refs_still_present
-  have sndgoal: "\<forall>rs. refs_of h' r rs \<longrightarrow> (\<forall>ref\<in>set rs. ref_present ref h')"
-    by (fastsimp elim!: crel_Ref_new dest: refs_of_is_fun)
+  have sndgoal: "\<forall>rs. refs_of h' r rs \<longrightarrow> (\<forall>ref\<in>set rs. Ref.present h' ref)"
+    by (fastsimp elim!: crel_ref dest: refs_of_is_fun)
   from fstgoal sndgoal show ?case ..
 qed
 
@@ -533,10 +533,10 @@ lemma rev'_simps [code]:
 thm arg_cong2
   by (auto simp add: expand_fun_eq intro: arg_cong2[where f = "op \<guillemotright>="] split: node.split)
 
-fun rev :: "('a:: heap) node \<Rightarrow> 'a node Heap" 
+primrec rev :: "('a:: heap) node \<Rightarrow> 'a node Heap" 
 where
   "rev Empty = return Empty"
-| "rev (Node x n) = (do q \<leftarrow> Ref.new Empty; p \<leftarrow> Ref.new (Node x n); v \<leftarrow> rev' (q, p); !v done)"
+| "rev (Node x n) = (do q \<leftarrow> ref Empty; p \<leftarrow> ref (Node x n); v \<leftarrow> rev' (q, p); !v done)"
 
 subsection {* Correctness Proof *}
 
@@ -556,17 +556,17 @@ next
   case (Cons x xs)
   (*"LinkedList.list_of h' (get_ref v h') (List.rev xs @ x # qsa)"*)
   from Cons(4) obtain ref where 
-    p_is_Node: "get_ref p h = Node x ref"
+    p_is_Node: "Ref.get h p = Node x ref"
     (*and "ref_present ref h"*)
     and list_of'_ref: "list_of' h ref xs"
-    unfolding list_of'_def by (cases "get_ref p h", auto)
-  from p_is_Node Cons(2) have crel_rev': "crel (rev' (p, ref)) (set_ref p (Node x q) h) h' v"
+    unfolding list_of'_def by (cases "Ref.get h p", auto)
+  from p_is_Node Cons(2) have crel_rev': "crel (rev' (p, ref)) (Ref.set p (Node x q) h) h' v"
     by (auto simp add: rev'_simps [of q p] elim!: crelE crel_lookup crel_update)
   from Cons(3) obtain qrs where qrs_def: "refs_of' h q qrs" by (elim list_of'_refs_of')
   from Cons(4) obtain prs where prs_def: "refs_of' h p prs" by (elim list_of'_refs_of')
   from qrs_def prs_def Cons(5) have distinct_pointers: "set qrs \<inter> set prs = {}" by fastsimp
   from qrs_def prs_def distinct_pointers refs_of'E have p_notin_qrs: "p \<notin> set qrs" by fastsimp
-  from Cons(3) qrs_def this have 1: "list_of' (set_ref p (Node x q) h) p (x#qs)"
+  from Cons(3) qrs_def this have 1: "list_of' (Ref.set p (Node x q) h) p (x#qs)"
     unfolding list_of'_def  
     apply (simp)
     unfolding list_of'_def[symmetric]
@@ -575,16 +575,16 @@ next
     unfolding refs_of'_def' by auto
   from prs_refs prs_def have p_not_in_refs: "p \<notin> set refs"
     by (fastsimp dest!: refs_of'_distinct)
-  with refs_def p_is_Node list_of'_ref have 2: "list_of' (set_ref p (Node x q) h) ref xs"
+  with refs_def p_is_Node list_of'_ref have 2: "list_of' (Ref.set p (Node x q) h) ref xs"
     by (auto simp add: list_of'_set_ref)
-  from p_notin_qrs qrs_def have refs_of1: "refs_of' (set_ref p (Node x q) h) p (p#qrs)"
+  from p_notin_qrs qrs_def have refs_of1: "refs_of' (Ref.set p (Node x q) h) p (p#qrs)"
     unfolding refs_of'_def'
     apply (simp)
     unfolding refs_of'_def'[symmetric]
     by (simp add: refs_of'_set_ref)
-  from p_not_in_refs p_is_Node refs_def have refs_of2: "refs_of' (set_ref p (Node x q) h) ref refs"
+  from p_not_in_refs p_is_Node refs_def have refs_of2: "refs_of' (Ref.set p (Node x q) h) ref refs"
     by (simp add: refs_of'_set_ref)
-  from p_not_in_refs refs_of1 refs_of2 distinct_pointers prs_refs have 3: "\<forall>qrs prs. refs_of' (set_ref p (Node x q) h) p qrs \<and> refs_of' (set_ref p (Node x q) h) ref prs \<longrightarrow> set prs \<inter> set qrs = {}"
+  from p_not_in_refs refs_of1 refs_of2 distinct_pointers prs_refs have 3: "\<forall>qrs prs. refs_of' (Ref.set p (Node x q) h) p qrs \<and> refs_of' (Ref.set p (Node x q) h) ref prs \<longrightarrow> set prs \<inter> set qrs = {}"
     apply - apply (rule allI)+ apply (rule impI) apply (erule conjE)
     apply (drule refs_of'_is_fun) back back apply assumption
     apply (drule refs_of'_is_fun) back back apply assumption
@@ -595,7 +595,7 @@ qed
 
 lemma rev_correctness:
   assumes list_of_h: "list_of h r xs"
-  assumes validHeap: "\<forall>refs. refs_of h r refs \<longrightarrow> (\<forall>r \<in> set refs. ref_present r h)"
+  assumes validHeap: "\<forall>refs. refs_of h r refs \<longrightarrow> (\<forall>r \<in> set refs. Ref.present h r)"
   assumes crel_rev: "crel (rev r) h h' r'"
   shows "list_of h' r' (List.rev xs)"
 using assms
@@ -606,39 +606,39 @@ proof (cases r)
 next
   case (Node x ps)
   with crel_rev obtain p q h1 h2 h3 v where
-    init: "crel (Ref.new Empty) h h1 q"
-    "crel (Ref.new (Node x ps)) h1 h2 p"
+    init: "crel (ref Empty) h h1 q"
+    "crel (ref (Node x ps)) h1 h2 p"
     and crel_rev':"crel (rev' (q, p)) h2 h3 v"
     and lookup: "crel (!v) h3 h' r'"
     using rev.simps
     by (auto elim!: crelE)
   from init have a1:"list_of' h2 q []"
     unfolding list_of'_def
-    by (auto elim!: crel_Ref_new)
+    by (auto elim!: crel_ref)
   from list_of_h obtain refs where refs_def: "refs_of h r refs" by (rule list_of_refs_of)
-  from validHeap init refs_def have heap_eq: "\<forall>refs. refs_of h r refs \<longrightarrow> (\<forall>ref\<in>set refs. ref_present ref h \<and> ref_present ref h2 \<and> get_ref ref h = get_ref ref h2)"
-    by (fastsimp elim!: crel_Ref_new dest: refs_of_is_fun)
+  from validHeap init refs_def have heap_eq: "\<forall>refs. refs_of h r refs \<longrightarrow> (\<forall>ref\<in>set refs. Ref.present h ref \<and> Ref.present h2 ref \<and> Ref.get h ref = Ref.get h2 ref)"
+    by (fastsimp elim!: crel_ref dest: refs_of_is_fun)
   from list_of_invariant[OF list_of_h heap_eq] have "list_of h2 r xs" .
   from init this Node have a2: "list_of' h2 p xs"
     apply -
     unfolding list_of'_def
-    apply (auto elim!: crel_Ref_new)
+    apply (auto elim!: crel_ref)
     done
   from init have refs_of_q: "refs_of' h2 q [q]"
-    by (auto elim!: crel_Ref_new)
+    by (auto elim!: crel_ref)
   from refs_def Node have refs_of'_ps: "refs_of' h ps refs"
     by (auto simp add: refs_of'_def'[symmetric])
-  from validHeap refs_def have all_ref_present: "\<forall>r\<in>set refs. ref_present r h" by simp
-  from init refs_of'_ps Node this have heap_eq: "\<forall>refs. refs_of' h ps refs \<longrightarrow> (\<forall>ref\<in>set refs. ref_present ref h \<and> ref_present ref h2 \<and> get_ref ref h = get_ref ref h2)"
-    by (fastsimp elim!: crel_Ref_new dest: refs_of'_is_fun)
+  from validHeap refs_def have all_ref_present: "\<forall>r\<in>set refs. Ref.present h r" by simp
+  from init refs_of'_ps Node this have heap_eq: "\<forall>refs. refs_of' h ps refs \<longrightarrow> (\<forall>ref\<in>set refs. Ref.present h ref \<and> Ref.present h2 ref \<and> Ref.get h ref = Ref.get h2 ref)"
+    by (fastsimp elim!: crel_ref dest: refs_of'_is_fun)
   from refs_of'_invariant[OF refs_of'_ps this] have "refs_of' h2 ps refs" .
   with init have refs_of_p: "refs_of' h2 p (p#refs)"
-    by (auto elim!: crel_Ref_new simp add: refs_of'_def')
+    by (auto elim!: crel_ref simp add: refs_of'_def')
   with init all_ref_present have q_is_new: "q \<notin> set (p#refs)"
-    by (auto elim!: crel_Ref_new intro!: noteq_refsI)
+    by (auto elim!: crel_ref intro!: Ref.noteq_I)
   from refs_of_p refs_of_q q_is_new have a3: "\<forall>qrs prs. refs_of' h2 q qrs \<and> refs_of' h2 p prs \<longrightarrow> set prs \<inter> set qrs = {}"
     by (fastsimp simp only: set.simps dest: refs_of'_is_fun)
-  from rev'_invariant [OF crel_rev' a1 a2 a3] have "list_of h3 (get_ref v h3) (List.rev xs)" 
+  from rev'_invariant [OF crel_rev' a1 a2 a3] have "list_of h3 (Ref.get h3 v) (List.rev xs)" 
     unfolding list_of'_def by auto
   with lookup show ?thesis
     by (auto elim: crel_lookup)
@@ -734,32 +734,32 @@ text {* From our original induction rule Lmerge.induct, we derive a new rule wit
 lemma merge_induct2:
   assumes "list_of' h (p::'a::{heap, ord} node ref) xs"
   assumes "list_of' h q ys"
-  assumes "\<And> ys p q. \<lbrakk> list_of' h p []; list_of' h q ys; get_ref p h = Empty \<rbrakk> \<Longrightarrow> P p q [] ys"
-  assumes "\<And> x xs' p q pn. \<lbrakk> list_of' h p (x#xs'); list_of' h q []; get_ref p h = Node x pn; get_ref q h = Empty \<rbrakk> \<Longrightarrow> P p q (x#xs') []"
+  assumes "\<And> ys p q. \<lbrakk> list_of' h p []; list_of' h q ys; Ref.get h p = Empty \<rbrakk> \<Longrightarrow> P p q [] ys"
+  assumes "\<And> x xs' p q pn. \<lbrakk> list_of' h p (x#xs'); list_of' h q []; Ref.get h p = Node x pn; Ref.get h q = Empty \<rbrakk> \<Longrightarrow> P p q (x#xs') []"
   assumes "\<And> x xs' y ys' p q pn qn.
-  \<lbrakk> list_of' h p (x#xs'); list_of' h q (y#ys'); get_ref p h = Node x pn; get_ref q h = Node y qn;
+  \<lbrakk> list_of' h p (x#xs'); list_of' h q (y#ys'); Ref.get h p = Node x pn; Ref.get h q = Node y qn;
   x \<le> y; P pn q xs' (y#ys') \<rbrakk>
   \<Longrightarrow> P p q (x#xs') (y#ys')"
   assumes "\<And> x xs' y ys' p q pn qn.
-  \<lbrakk> list_of' h p (x#xs'); list_of' h q (y#ys'); get_ref p h = Node x pn; get_ref q h = Node y qn;
+  \<lbrakk> list_of' h p (x#xs'); list_of' h q (y#ys'); Ref.get h p = Node x pn; Ref.get h q = Node y qn;
   \<not> x \<le> y; P p qn (x#xs') ys'\<rbrakk>
   \<Longrightarrow> P p q (x#xs') (y#ys')"
   shows "P p q xs ys"
 using assms(1-2)
 proof (induct xs ys arbitrary: p q rule: Lmerge.induct)
   case (2 ys)
-  from 2(1) have "get_ref p h = Empty" unfolding list_of'_def by simp
+  from 2(1) have "Ref.get h p = Empty" unfolding list_of'_def by simp
   with 2(1-2) assms(3) show ?case by blast
 next
   case (3 x xs')
-  from 3(1) obtain pn where Node: "get_ref p h = Node x pn" by (rule list_of'_Cons)
-  from 3(2) have "get_ref q h = Empty" unfolding list_of'_def by simp
+  from 3(1) obtain pn where Node: "Ref.get h p = Node x pn" by (rule list_of'_Cons)
+  from 3(2) have "Ref.get h q = Empty" unfolding list_of'_def by simp
   with Node 3(1-2) assms(4) show ?case by blast
 next
   case (1 x xs' y ys')
-  from 1(3) obtain pn where pNode:"get_ref p h = Node x pn"
+  from 1(3) obtain pn where pNode:"Ref.get h p = Node x pn"
     and list_of'_pn: "list_of' h pn xs'" by (rule list_of'_Cons)
-  from 1(4) obtain qn where qNode:"get_ref q h = Node y qn"
+  from 1(4) obtain qn where qNode:"Ref.get h q = Node y qn"
     and  list_of'_qn: "list_of' h qn ys'" by (rule list_of'_Cons)
   show ?case
   proof (cases "x \<le> y")
@@ -780,15 +780,15 @@ lemma merge_induct3:
 assumes  "list_of' h p xs"
 assumes  "list_of' h q ys"
 assumes  "crel (merge p q) h h' r"
-assumes  "\<And> ys p q. \<lbrakk> list_of' h p []; list_of' h q ys; get_ref p h = Empty \<rbrakk> \<Longrightarrow> P p q h h q [] ys"
-assumes  "\<And> x xs' p q pn. \<lbrakk> list_of' h p (x#xs'); list_of' h q []; get_ref p h = Node x pn; get_ref q h = Empty \<rbrakk> \<Longrightarrow> P p q h h p (x#xs') []"
+assumes  "\<And> ys p q. \<lbrakk> list_of' h p []; list_of' h q ys; Ref.get h p = Empty \<rbrakk> \<Longrightarrow> P p q h h q [] ys"
+assumes  "\<And> x xs' p q pn. \<lbrakk> list_of' h p (x#xs'); list_of' h q []; Ref.get h p = Node x pn; Ref.get h q = Empty \<rbrakk> \<Longrightarrow> P p q h h p (x#xs') []"
 assumes  "\<And> x xs' y ys' p q pn qn h1 r1 h'.
-  \<lbrakk> list_of' h p (x#xs'); list_of' h q (y#ys');get_ref p h = Node x pn; get_ref q h = Node y qn;
-  x \<le> y; crel (merge pn q) h h1 r1 ; P pn q h h1 r1 xs' (y#ys'); h' = set_ref p (Node x r1) h1 \<rbrakk>
+  \<lbrakk> list_of' h p (x#xs'); list_of' h q (y#ys');Ref.get h p = Node x pn; Ref.get h q = Node y qn;
+  x \<le> y; crel (merge pn q) h h1 r1 ; P pn q h h1 r1 xs' (y#ys'); h' = Ref.set p (Node x r1) h1 \<rbrakk>
   \<Longrightarrow> P p q h h' p (x#xs') (y#ys')"
 assumes "\<And> x xs' y ys' p q pn qn h1 r1 h'.
-  \<lbrakk> list_of' h p (x#xs'); list_of' h q (y#ys'); get_ref p h = Node x pn; get_ref q h = Node y qn;
-  \<not> x \<le> y; crel (merge p qn) h h1 r1; P p qn h h1 r1 (x#xs') ys'; h' = set_ref q (Node y r1) h1 \<rbrakk>
+  \<lbrakk> list_of' h p (x#xs'); list_of' h q (y#ys'); Ref.get h p = Node x pn; Ref.get h q = Node y qn;
+  \<not> x \<le> y; crel (merge p qn) h h1 r1; P p qn h h1 r1 (x#xs') ys'; h' = Ref.set q (Node y r1) h1 \<rbrakk>
   \<Longrightarrow> P p q h h' q (x#xs') (y#ys')"
 shows "P p q h h' r xs ys"
 using assms(3)
@@ -808,7 +808,7 @@ next
   case (3 x xs' y ys' p q pn qn)
   from 3(3-5) 3(7) obtain h1 r1 where
     1: "crel (merge pn q) h h1 r1" 
-    and 2: "h' = set_ref p (Node x r1) h1 \<and> r = p"
+    and 2: "h' = Ref.set p (Node x r1) h1 \<and> r = p"
     unfolding merge_simps[of p q]
     by (auto elim!: crel_lookup crelE crel_return crel_if crel_update)
   from 3(6)[OF 1] assms(6) [OF 3(1-5)] 1 2 show ?case by simp
@@ -816,7 +816,7 @@ next
   case (4 x xs' y ys' p q pn qn)
   from 4(3-5) 4(7) obtain h1 r1 where
     1: "crel (merge p qn) h h1 r1" 
-    and 2: "h' = set_ref q (Node y r1) h1 \<and> r = q"
+    and 2: "h' = Ref.set q (Node y r1) h1 \<and> r = q"
     unfolding merge_simps[of p q]
     by (auto elim!: crel_lookup crelE crel_return crel_if crel_update)
   from 4(6)[OF 1] assms(7) [OF 4(1-5)] 1 2 show ?case by simp
@@ -834,7 +834,7 @@ lemma merge_unchanged:
   assumes "crel (merge p q) h h' r'"
   assumes "set xs \<inter> set ys = {}"
   assumes "r \<notin> set xs \<union> set ys"
-  shows "get_ref r h = get_ref r h'"
+  shows "Ref.get h r = Ref.get h' r"
 proof -
   from assms(1) obtain ps where ps_def: "list_of' h p ps" by (rule refs_of'_list_of')
   from assms(2) obtain qs where qs_def: "list_of' h q qs" by (rule refs_of'_list_of')
@@ -853,7 +853,8 @@ proof -
     from pnrs_def 3(12) have "r \<noteq> p" by auto
     with 3(11) 3(12) pnrs_def refs_of'_distinct[OF 3(9)] have p_in: "p \<notin> set pnrs \<union> set ys" by auto
     from 3(11) pnrs_def have no_inter: "set pnrs \<inter> set ys = {}" by auto
-    from 3(7)[OF refs_of'_pn 3(10) this p_in] 3(3) have p_is_Node: "get_ref p h1 = Node x pn" by simp
+    from 3(7)[OF refs_of'_pn 3(10) this p_in] 3(3) have p_is_Node: "Ref.get h1 p = Node x pn"
+      by simp
     from 3(7)[OF refs_of'_pn 3(10) no_inter r_in] 3(8) `r \<noteq> p` show ?case
       by simp
   next
@@ -866,7 +867,7 @@ proof -
     from qnrs_def 4(12) have "r \<noteq> q" by auto
     with 4(11) 4(12) qnrs_def refs_of'_distinct[OF 4(10)] have q_in: "q \<notin> set xs \<union> set qnrs" by auto
     from 4(11) qnrs_def have no_inter: "set xs \<inter> set qnrs = {}" by auto
-    from 4(7)[OF 4(9) refs_of'_qn this q_in] 4(4) have q_is_Node: "get_ref q h1 = Node y qn" by simp
+    from 4(7)[OF 4(9) refs_of'_qn this q_in] 4(4) have q_is_Node: "Ref.get h1 q = Node y qn" by simp
     from 4(7)[OF 4(9) refs_of'_qn no_inter r_in] 4(8) `r \<noteq> q` show ?case
       by simp
   qed
@@ -899,7 +900,7 @@ proof -
       by (rule refs_of'_Node)
     from 3(10) 3(9) 3(11) pnrs_def refs_of'_distinct[OF 3(9)] have p_in: "p \<notin> set pnrs \<union> set ys" by auto
     from 3(11) pnrs_def have no_inter: "set pnrs \<inter> set ys = {}" by auto
-    from merge_unchanged[OF refs_of'_pn 3(10) 3(6) no_inter p_in] have p_stays: "get_ref p h1 = get_ref p h" ..
+    from merge_unchanged[OF refs_of'_pn 3(10) 3(6) no_inter p_in] have p_stays: "Ref.get h1 p = Ref.get h p" ..
     from 3 p_stays obtain r1s
       where rs_def: "rs = p#r1s" and refs_of'_r1:"refs_of' h1 r1 r1s"
       by (auto elim: refs_of'_set_next_ref)
@@ -912,7 +913,7 @@ proof -
       by (rule refs_of'_Node)
     from 4(10) 4(9) 4(11) qnrs_def refs_of'_distinct[OF 4(10)] have q_in: "q \<notin> set xs \<union> set qnrs" by auto
     from 4(11) qnrs_def have no_inter: "set xs \<inter> set qnrs = {}" by auto
-    from merge_unchanged[OF 4(9) refs_of'_qn 4(6) no_inter q_in] have q_stays: "get_ref q h1 = get_ref q h" ..
+    from merge_unchanged[OF 4(9) refs_of'_qn 4(6) no_inter q_in] have q_stays: "Ref.get h1 q = Ref.get h q" ..
     from 4 q_stays obtain r1s
       where rs_def: "rs = q#r1s" and refs_of'_r1:"refs_of' h1 r1 r1s"
       by (auto elim: refs_of'_set_next_ref)
@@ -945,7 +946,7 @@ next
   from prs_def qrs_def 3(9) pnrs_def have no_inter: "set pnrs \<inter> set qrs = {}" by fastsimp
   from no_inter refs_of'_pn qrs_def have no_inter2: "\<forall>qrs prs. refs_of' h q qrs \<and> refs_of' h pn prs \<longrightarrow> set prs \<inter> set qrs = {}"
     by (fastsimp dest: refs_of'_is_fun)
-  from merge_unchanged[OF refs_of'_pn qrs_def 3(6) no_inter p_in] have p_stays: "get_ref p h1 = get_ref p h" ..
+  from merge_unchanged[OF refs_of'_pn qrs_def 3(6) no_inter p_in] have p_stays: "Ref.get h1 p = Ref.get h p" ..
   from 3(7)[OF no_inter2] obtain rs where rs_def: "refs_of' h1 r1 rs" by (rule list_of'_refs_of')
   from refs_of'_merge[OF refs_of'_pn qrs_def 3(6) no_inter this] p_in have p_rs: "p \<notin> set rs" by auto
   with 3(7)[OF no_inter2] 3(1-5) 3(8) p_rs rs_def p_stays
@@ -962,7 +963,7 @@ next
   from prs_def qrs_def 4(9) qnrs_def have no_inter: "set prs \<inter> set qnrs = {}" by fastsimp
   from no_inter refs_of'_qn prs_def have no_inter2: "\<forall>qrs prs. refs_of' h qn qrs \<and> refs_of' h p prs \<longrightarrow> set prs \<inter> set qrs = {}"
     by (fastsimp dest: refs_of'_is_fun)
-  from merge_unchanged[OF prs_def refs_of'_qn 4(6) no_inter q_in] have q_stays: "get_ref q h1 = get_ref q h" ..
+  from merge_unchanged[OF prs_def refs_of'_qn 4(6) no_inter q_in] have q_stays: "Ref.get h1 q = Ref.get h q" ..
   from 4(7)[OF no_inter2] obtain rs where rs_def: "refs_of' h1 r1 rs" by (rule list_of'_refs_of')
   from refs_of'_merge[OF prs_def refs_of'_qn 4(6) no_inter this] q_in have q_rs: "q \<notin> set rs" by auto
   with 4(7)[OF no_inter2] 4(1-5) 4(8) q_rs rs_def q_stays
@@ -984,8 +985,8 @@ definition test_3 where "test_3 =
   (do
     ll_xs \<leftarrow> make_llist (filter (%n. n mod 2 = 0) [2..8]);
     ll_ys \<leftarrow> make_llist (filter (%n. n mod 2 = 1) [5..11]);
-    r \<leftarrow> Ref.new ll_xs;
-    q \<leftarrow> Ref.new ll_ys;
+    r \<leftarrow> ref ll_xs;
+    q \<leftarrow> ref ll_ys;
     p \<leftarrow> merge r q;
     ll_zs \<leftarrow> !p;
     zs \<leftarrow> traverse ll_zs;
